FiatFormal/Language/TyJudge.v
@@ -6,46 +6,47 @@ Require Export FiatFormal.Language.Exp.
 
 
 (* Type judgement assigns a type to an expression. *)
-Inductive TYPE : kienv -> tyenv -> exp -> ty -> Prop :=
+Inductive TYPE : defs -> kienv -> tyenv -> exp -> ty -> Prop :=
  | TYVar
-   :  forall i ke te t
-   ,  get i te = Some t
+   :  forall i ds ke te t,
+     get i te = Some t
    -> KIND ke t  KStar
-   -> TYPE ke te (XVar i) t
+   -> TYPE ds ke te (XVar i) t
 
  | TYLam
-   :  forall ke te x12 t11 t12
-   ,  KIND ke t11 KStar
-   -> TYPE ke (te :> t11)  x12            t12
-   -> TYPE ke  te         (XLam t11 x12) (TFun t11 t12)
+   :  forall ds ke te x12 t11 t12,
+     KIND ke t11 KStar
+   -> TYPE ds ke (te :> t11)  x12            t12
+   -> TYPE ds ke  te         (XLam t11 x12) (TFun t11 t12)
 
  | TYApp
-   :  forall ke te x1 x2 t11 t12
-   ,  TYPE ke te x1 (TFun t11 t12)
-   -> TYPE ke te x2 t11
-   -> TYPE ke te (XApp x1 x2) t12
+   :  forall ds ke te x1 x2 t11 t12,
+     TYPE ds ke te x1 (TFun t11 t12)
+   -> TYPE ds ke te x2 t11
+   -> TYPE ds ke te (XApp x1 x2) t12
 
  | TYTup
-   : forall ke te xs ts,
-     Forall2 (TYPE ke te) xs ts
-     -> TYPE ke te (XTup xs) (TNProd ts)
+   : forall ds ke te xs ts,
+     Forall2 (TYPE ds ke te) xs ts
+     -> TYPE ds ke te (XTup xs) (TNProd ts)
 
  | TYNFun
-   : forall ke te x ts tRes,
-     TYPE ke (te >< ts) x tRes
-     -> TYPE ke te (XNFun ts x) (TNFun ts tRes)
+   : forall ds ke te x ts tRes,
+     Forall (fun t => KIND ke t KStar) ts
+     -> TYPE ds ke (te >< ts) x tRes
+     -> TYPE ds ke te (XNFun ts x) (TNFun ts tRes)
 
  | TYProj
-   : forall ke te n x ts tRes,
-     TYPE ke te x (TNProd ts)
+   : forall ds ke te n x ts tRes,
+     TYPE ds ke te x (TNProd ts)
      -> get n ts = Some tRes
-     -> TYPE ke te (XProj n x) tRes
+     -> TYPE ds ke te (XProj n x) tRes
 
  | TYNApp
-   : forall ke te x xArgs ts tRes,
-     TYPE ke te x (TNFun ts tRes)
-     -> Forall2 (TYPE ke te) xArgs ts
-     -> TYPE ke te (XNApp x xArgs) tRes
+   : forall ds ke te x xArgs ts tRes,
+     TYPE ds ke te x (TNFun ts tRes)
+     -> Forall2 (TYPE ds ke te) xArgs ts
+     -> TYPE ds ke te (XNApp x xArgs) tRes
 
  (* | TYLAM *)
  (*   :  forall ke te x1 t1 *)
@@ -56,116 +57,296 @@ Inductive TYPE : kienv -> tyenv -> exp -> ty -> Prop :=
  (*   :  forall ke te x1 t1 t2 *)
  (*   ,  TYPE ke te x1 (TForall t1) *)
  (*   -> KIND ke t2 KStar *)
- (*   -> TYPE ke te (XAPP x1 t2) (substTT 0 t2 t1) *).
+ (*   -> TYPE ke te (XAPP x1 t2) (substTT 0 t2 t1) *)
+
+ | TYFix
+   : forall ds ke te t1 t2 x,
+     KIND ke t1 KStar
+     -> TYPE ds ke (te :> (TFun t1 t2) :> t1) x t2
+     -> TYPE ds ke te (XFix t1 t2 x) (TFun t1 t2)
+
+ | TYCon
+   : forall ds ke te dc xs tsArgs tc dcs,
+     getDataDef dc ds = Some (DefData dc tsArgs (TCon tc))
+     -> getTypeDef tc ds = Some (DefDataType tc dcs)
+     -> Forall (simpleType) tsArgs
+     -> In dc dcs
+     -> Forall2 (TYPE ds ke te) xs tsArgs
+     -> TYPE ds ke te (XCon dc xs) (TCon tc)
+
+ (* Case Expressions *)
+ | TYMatch
+   : forall ds ke te xObj tcPat tRes alts dcs,
+     (* check types of expression and alternatives *)
+     TYPE ds ke te xObj (TCon tcPat)
+     -> Forall (fun alt => TYPEA ds ke te alt (TCon tcPat) tRes) alts
+     (* there must be at least one alternative *)
+     -> length alts > 0
+     (* all data cons must have a corresponding alternative *)
+     -> getTypeDef tcPat ds = Some (DefDataType tcPat dcs)
+     -> Forall (fun dc => In dc (map dcOfAlt alts)) dcs
+     -> TYPE ds ke te (XMatch xObj alts) tRes
+
+with TYPEA : defs -> kienv -> tyenv -> alt -> ty -> ty -> Prop :=
+ | TYAlt
+   : forall ds ke te x1 t1 dc tsArgs tcPat,
+     getDataDef dc ds = Some (DefData dc tsArgs (TCon tcPat))
+     -> Forall (simpleType) tsArgs
+     (* note: checking tRes well kinded is implicit in TYMatch, I *)
+     (* believe *)
+     (* note: currently there is no such KIND premise in TYCon, which seems wrongly asymmetric *)
+     -> Forall (fun t => KIND ke t KStar) tsArgs
+     -> TYPE  ds ke (te >< tsArgs) x1 t1
+     -> TYPEA ds ke te (AAlt dc tsArgs x1) (TCon tcPat) t1.
 
 Hint Constructors TYPE.
+Hint Constructors TYPEA.
+
+
+(* -------------------------------------------------- *)
 
 (* ADT judgement assigns a type to an ADT. *)
-Inductive TYPEADT : kienv -> tyenv -> adt -> ty -> Prop :=
-| TYADT : forall ke te x τr τ,
+Inductive TYPEADT : defs -> kienv -> tyenv -> adt -> ty -> Prop :=
+| TYADT : forall ds ke te x τr τ,
     KIND ke τr KStar
     (* -> KIND (ke :> KStar) τ *)
     (* KStar *) (* decided this wasn't necessary since in presence of following premise *)
     (* ADT method bodies type according to signatures *)
-    -> TYPE ke te x (substTT 0 τr τ)
+    -> TYPE ds ke te x (substTT 0 τr τ)
     (* -> t = TNProd ts ... add this later, also think about how to *)
     (* enforce type of each element in the product *)
-    -> TYPEADT ke te (IADT τr x (TExists τ)) (TExists τ).
+    -> TYPEADT ds ke te (IADT τr x (TExists τ)) (TExists τ).
 Hint Constructors TYPEADT.
 
 (* Program judgement assigns a type to a program. *)
-Inductive TYPEPROG : kienv -> tyenv -> prog -> ty -> Prop :=
-| TYLet : forall ke te τr x τ p t2,
-    TYPEADT ke te (IADT τr x (TExists τ)) (TExists τ)
-    -> TYPEPROG (ke :> KStar) ((liftTE 0 te) :> τ) p t2
-    -> TYPEPROG ke te (PLET (IADT τr x (TExists τ)) p) (substTT 0 τr t2)
-| TYExp : forall ke te x t,
-    TYPE ke te x t
-    -> TYPEPROG ke te (PEXP x) t.
+Inductive TYPEPROG : defs -> kienv -> tyenv -> prog -> ty -> Prop :=
+| TYLet : forall ds ke te τr x τ p t2,
+    TYPEADT ds ke te (IADT τr x (TExists τ)) (TExists τ)
+    -> TYPEPROG ds (ke :> KStar) ((liftTE 0 te) :> τ) p t2
+    -> TYPEPROG ds ke te (PLET (IADT τr x (TExists τ)) p) (substTT 0 τr t2)
+| TYExp : forall ds ke te x t,
+    TYPE ds ke te x t
+    -> TYPEPROG ds ke te (PEXP x) t.
 
 Ltac invert_adt_type :=
   repeat
     (match goal with
-     | [ H : TYPEADT _ _ ?a _ |- _ ] => destruct a; inverts keep H
+     | [ H : TYPEADT _ _ _ ?a _ |- _ ] => destruct a; inverts H
      end).
 
 Ltac invert_exp_type :=
   repeat
     (match goal with
-     | [ H : TYPE _ _ _ _ |- _] => inverts keep H
+     | [ H: TYPE  _ _ _ (XVar  _)     _    |- _ ] => inverts H
+     | [ H: TYPE  _ _ _ (XLam  _ _)   _    |- _ ] => inverts H
+     | [ H: TYPE  _ _ _ (XApp  _ _)   _    |- _ ] => inverts H
+     | [ H: TYPE  _ _ _ (XTup _)   _    |- _ ] => inverts H
+     | [ H: TYPE  _ _ _ (XProj  _ _)   _    |- _ ] => inverts H
+     | [ H: TYPE  _ _ _ (XFix  _ _ _)   _    |- _ ] => inverts H
+     | [ H: TYPE  _ _ _ (XNFun _ _)   _    |- _ ] => inverts H
+     | [ H: TYPE  _ _ _ (XNApp  _ _)   _    |- _ ] => inverts H
+     | [ H: TYPE  _ _ _ (XCon _ _) _    |- _ ] => inverts H
+     | [ H: TYPE  _ _ _ (XMatch _ _)   _    |- _ ] => inverts H
+     | [ H: TYPEA _ _ _ (AAlt _ _ _)    _ _  |- _ ] => inverts H
     end).
 
 Ltac invert_prog_type :=
   repeat
     (match goal with
-     | [ H : TYPEPROG _ _ _ _ |- _] => inverts keep H
+     | [ H : TYPEPROG _ _ _ _ _ |- _] => inverts H
     end).
 
 Ltac inverts_type :=
   repeat
     (match goal with
-     | [ H : TYPE _ _ _ _ |- _ ] => inverts keep H
-     | [ H : TYPEADT _ _ _ _ |- _ ] => inverts keep H
-     | [ H : TYPEPROG _ _ _ _ |- _ ] => inverts keep H
+     | [ H : TYPE _ _ _ _ _ |- _ ] => inverts H
+     | [ H : TYPEADT _ _ _ _ _ |- _ ] => inverts H
+     | [ H : TYPEPROG _ _ _ _ _ |- _ ] => inverts H
      end).
+
+
+Lemma Forall2_exists_right_in
+ : forall {A B} (R: A -> B -> Prop) y xs ys
+ ,             In y ys  -> Forall2 R xs ys
+ -> (exists x, In x xs  /\         R x  y).
+Proof.
+ intros.
+ induction H0.
+  false.
+  simpl in H. destruct H.
+   subst.
+   exists x. split. simpl. auto. auto.
+   lets D: IHForall2 H.
+   destruct D.
+   exists x0.
+    inverts H2.
+    split. simpl. auto. auto.
+Qed.
 
 (* ----------------------------------------------------- *)
 (* The type produced by a type judgement is well kinded. *)
 Theorem type_kind
- :  forall ke te x t
- ,  TYPE ke te x t
- -> KIND ke t KStar.
+  : forall ds ke te x t,
+    TYPE ds ke te x t
+    -> KIND ke t KStar.
 Proof.
- intros. gen ke te t.
- induction x; intros; inverts H; eauto.
+ intros. gen ds ke te t.
+ induction x using exp_mutind
+   with (PA := fun a => forall ds ke te tBuilds tRes,
+                   TYPEA ds ke te a tBuilds tRes
+                   -> KIND ke tRes KStar); intros; try (first [inverts H | inverts H0]); eauto.
 
  (* Case "XAPP". *)
  (*  apply IHx in H4. inverts H4. *)
  (*  eapply subst_type_type; eauto. *)
 
  Case "XLam".
-  eapply IHx1 in H4. inverts H4. auto.
+ eapply IHx1 in H5. inverts H5. auto.
 
-  Case "XTup".
+ Case "XTup".
+ inverts H0. inverts H4.
+ apply KINProd; auto.
+ inverts keep H0.
+ inverts keep H6.
+ apply KINProd. apply Forall_cons.
+ eapply H1; eauto.
+ rewrite Forall_forall; intros.
+ rename x0 into t.
+ rename l0 into xs.
+ nforall.
+ pose proof (Forall2_exists_right_in _ _ _ _ H H7) as [x' [INx' TYx']].
+ spec H2 INx' TYx'; auto.
 
-  apply KINProd.
+ Case "XProj".
+ spec IHx H5.
+ inverts_kind.
+ nforall.
+ pose proof (get_in _ _ _ _ H7).
+ spec H1 H; auto.
+
+ Case "XNApp".
+ inverts keep H0.
+ inverts keep H7.
+ spec IHx H5. inverts_kind; auto.
+ inverts keep H0.
+ spec IHx H7.
+ inverts_kind; auto.
+
+ Case "XCon".
+ inverts H0; auto.
+ inverts H0; auto.
+
+ Case "XMatch".
+ inverts keep H0; nope.
+ inverts keep H0.
+ repeat nforall.
+ spec H5 x0.
+ assert (In x0 (l0 :> x0)) by auto.
+ spec H5 H. spec H1 H5; auto.
 Qed.
+
+
+(* Ltac stomp_forall := *)
+(*   do 1 (first [ inverts_type | *)
+(*                 nforall | *)
+(*                 constructor | *)
+(*                 rewrite Forall_forall; intros | *)
+(*                 eauto ]). *)
 
 
 (* A well typed expression is well formed. *)
 Theorem type_wfX
- :  forall ke te x t
- ,  TYPE ke te x t
- -> wfX  ke te x.
+  : forall ds ke te x t,
+    TYPE ds ke te x t
+    -> wfX ke te x.
 Proof.
- intros. gen ke te t.
- induction x; intros; simpl.
+  intros. gen ds ke te t.
+  induction x using exp_mutind
+    with (PA := fun a => forall ds ke te tBuilds tRes,
+                    TYPEA ds ke te a tBuilds tRes
+                    -> wfA ke te a); intros; simpl.
 
- Case "XVar".
+  Case "XVar".
   inverts H. eauto.
 
- (* Case "XLAM". *)
- (*  inverts H. *)
- (*  apply IHx in H3. eauto. *)
+  (* Case "XLAM". *)
+  (*  inverts H. *)
+  (*  apply IHx in H3. eauto. *)
 
- (* Case "XAPP". *)
- (*  inverts H. *)
- (*  lets D: IHx H4. split. *)
- (*   auto. eapply kind_wfT. eauto. *)
+  (* Case "XAPP". *)
+  (*  inverts H. *)
+  (*  lets D: IHx H4. split. *)
+  (*   auto. eapply kind_wfT. eauto. *)
 
- Case "XLam".
+  Case "XLam".
   inverts H.
-  apply IHx in H6.
-  apply kind_wfT in H4. auto.
+  apply IHx in H7.
+  apply kind_wfT in H5. auto.
 
- Case "XApp".
+  Case "XApp".
   inverts H.
-  apply IHx1 in H4.
-  apply IHx2 in H6.
-   auto.
+  apply IHx1 in H5.
+  apply IHx2 in H7.
+  auto.
+
+  Case "XTup".
+  inverts keep H0.
+  nforall.
+  constructor.
+  rewrite Forall_forall; intros.
+  pose proof (Forall2_exists_left_in _ _ _ _ H1 H5) as [y [INy TYx]].
+  eapply H; eauto.
+
+  Case "XProj".
+  inverts keep H.
+  constructor. eapply IHx.
+  eauto.
+
+  Case "XNFun".
+  inverts keep H.
+  constructor.
+  apply Forall_forall; intros.
+  nforall. spec H5 H0.
+  eapply kind_wfT; eauto.
+  spec IHx H7; auto.
+
+  Case "XNApp".
+  inverts keep H0.
+  spec IHx H6.
+  constructor; auto.
+  rewrite Forall_forall; intros.
+  repeat nforall.
+  spec H H1.
+  pose proof (Forall2_exists_left_in _ _ _ _ H1 H8) as [y [INy TYx]].
+  eapply H; eauto.
+
+  Case "XFix".
+  inverts keep H.
+  constructor.
+  eapply kind_wfT; eauto.
+  pose proof (type_kind _ _ _ _ _ H).
+  inverts_kind. eapply kind_wfT; eauto.
+  eapply IHx; eauto.
+
+  Case "XCon". (* similar to XTup case, target for automation *)
+  inverts keep H0.
+  constructor.
+  repeat nforall. intros.
+  pose proof (Forall2_exists_left_in _ _ _ _ H1 H11) as [y [INy TYx]].
+  eapply H; eauto.
+
+  Case "XMatch".
+  inverts keep H0.
+  repeat nforall.
+  constructor.
+  eapply IHx; eauto.
+  rewrite Forall_forall; intros.
+  spec H H1. spec H4 H1. spec H H4; auto.
+  inverts keep H. econstructor; eauto.
 Qed.
 Hint Resolve type_wfX.
 
+(* AUTOMATION! *)
 
 (********************************************************************)
 (* Weakening the kind environment of a type judgement.
@@ -178,48 +359,149 @@ Hint Resolve type_wfX.
    resulting type -- so we must lift all of them.
  *)
 Lemma type_kienv_insert
- :  forall ix ke te x1 t1 k2
- ,  TYPE ke                 te             x1             t1
- -> TYPE (insert ix k2 ke) (liftTE ix te) (liftTX ix x1) (liftTT ix t1).
+  : forall ix ds ke te x1 t1 k2,
+    TYPE ds ke te x1 t1
+ -> TYPE ds (insert ix k2 ke) (liftTE ix te) (liftTX ix x1) (liftTT ix t1).
 Proof.
- intros. gen ix ke te t1 k2.
- induction x1; intros; inverts H; simpl; eauto.
+  intros. gen ix ds ke te t1 k2.
+  induction x1 using exp_mutind
+    with (PA := fun a => forall ix ds ke te tBuilds tRes k2,
+                    TYPEA ds ke te a tBuilds tRes
+                    -> TYPEA ds (insert ix k2 ke) (liftTE ix te) (liftTA ix a)
+                            (liftTT ix tBuilds) (liftTT ix tRes));
+    intros; invert_exp_type; simpl; eauto.
 
- Case "XVar".
+  Case "XVar".
   apply TYVar.
   apply get_map. auto.
   apply liftTT_insert. auto.
 
- (* Case "XLAM". *)
- (*  eapply TYLAM. *)
- (*  rewrite insert_rewind. *)
- (*   rewrite (liftTE_liftTE 0 ix). *)
- (*   apply IHx1. auto. *)
+  (* Case "XLAM". *)
+  (*  eapply TYLAM. *)
+  (*  rewrite insert_rewind. *)
+  (*   rewrite (liftTE_liftTE 0 ix). *)
+  (*   apply IHx1. auto. *)
 
- (* Case "XAPP". *)
- (*  rewrite (liftTT_substTT' 0 ix). simpl. *)
- (*  eapply TYAPP. *)
- (*  eapply (IHx1 ix) in H4. simpl in H4. eauto. *)
- (*  apply liftTT_insert. auto. *)
+  (* Case "XAPP". *)
+  (*  rewrite (liftTT_substTT' 0 ix). simpl. *)
+  (*  eapply TYAPP. *)
+  (*  eapply (IHx1 ix) in H4. simpl in H4. eauto. *)
+  (*  apply liftTT_insert. auto. *)
 
- Case "XLam".
+  Case "XLam".
   apply TYLam.
-   apply liftTT_insert. auto.
-   assert ( liftTE ix te :> liftTT ix t
-          = liftTE ix (te :> t)). auto. rewrite H. clear H.
-   apply IHx1. auto.
+  apply liftTT_insert. auto.
+  assert ( liftTE ix te :> liftTT ix t
+           = liftTE ix (te :> t)). auto. rewrite H. clear H.
+  apply IHx1. auto.
 
- Case "XApp".
+  Case "XApp".
   eapply TYApp.
-   eapply IHx1_1 in H4. simpl in H4. eauto.
-   eapply IHx1_2 in H6. eauto.
+  eapply IHx1_1 in H5. simpl in H5. eauto.
+  eapply IHx1_2 in H7. eauto.
+
+  Case "XTup".
+  eapply TYTup; simpl; auto.
+  apply (Forall2_map_left (TYPE ds (insert ix k2 ke) (liftTE ix te))).
+  apply (Forall2_map_right (fun (x : exp) (y : ty) => TYPE ds (insert ix k2 ke) (liftTE ix te) (liftTX ix x) y)).
+  apply (Forall2_impl_in  (TYPE ds ke te)); eauto.
+  nforall. intros.
+  eapply H; eauto.
+
+  Case "XProj".
+  eapply TYProj; simpl; eauto.
+  spec IHx1 H5. simpl in *; eauto.
+
+  Case "XNFun".
+  eapply TYNFun; eauto.
+  apply Forall_map.
+  repeat nforall; intros.
+  apply liftTT_insert; auto.
+  spec IHx1 H7.
+  unfold liftTE in *.
+  rewrite <- map_app; eauto.
+
+  Case "XNApp".
+  apply TYNApp with (ts := map (liftTT ix) ts).
+  assert (liftTT ix (TNFun ts t1) = (TNFun (map (liftTT ix) ts) (liftTT ix t1))) by auto.
+  rewrite <- H0.
+  apply IHx1; auto.
+
+  apply (Forall2_map_left (TYPE ds (insert ix k2 ke) (liftTE ix te))).
+  apply (Forall2_map_right (fun (x : exp) (y : ty) => TYPE ds (insert ix k2 ke) (liftTE ix te) (liftTX ix x) y)).
+  apply (Forall2_impl_in  (TYPE ds ke te)); eauto.
+  nforall. intros.
+  eapply H; eauto.
+
+  Case "XFix".
+  eapply TYFix. apply liftTT_insert; auto.
+  unfold liftTE in *.
+  assert (liftTT ix (TFun t1 t2) = (TFun (liftTT ix t1) (liftTT ix t2))) by auto.
+  rewrite <- H.
+  repeat rewrite <- map_cons.
+  apply IHx1; auto.
+
+  Case "XCon".
+  eapply TYCon; eauto.
+  apply (Forall2_map_left (TYPE ds (insert ix k2 ke) (liftTE ix te))).
+  apply (Forall2_impl_in  (TYPE ds ke te)); eauto.
+  nforall; eauto.
+  intros. spec H5 H1.
+  assert (y = liftTT ix y).
+  apply simpleLiftEq; auto.
+  rewrite H6.
+  nforall.
+  apply H; auto.
+
+  Case "XMatch".
+  eapply TYMatch; eauto.
+  assert (TCon tcPat = (liftTT ix (TCon tcPat))) by auto.
+  rewrite H0.
+  apply IHx1; auto.
+
+  apply Forall_map.
+  apply (Forall_impl_in (fun a => TYPEA ds ke te a (TCon tcPat) t1)); eauto.
+  repeat nforall; intros.
+  spec H H0. spec H H1. eauto.
+  rewrite map_length; auto.
+
+  (* norm. *) repeat nforall.
+  intros. rename x into d.
+  rewrite map_map. unfold Basics.compose.
+  eapply map_exists_in.
+  have (In d (map dcOfAlt aa)).
+  assert (exists a, dcOfAlt a = d /\ In a aa).
+  eapply map_in_exists. auto.
+  shift a. rip.
+  eapply dcOfAlt_liftTA.
+
+  Case "XAlt".
+  eapply TYAlt; eauto.
+  assert (map (liftTT ix) ts = ts).
+  repeat nforall. rewrite <- map_id.
+  apply map_ext_in; intros. symmetry.
+  spec H7 H.
+  apply (simpleLiftEq _ _ H7).
+  rewrite H; auto.
+  pose proof (simpleLiftMapEq _ ix H7).
+  rewrite <- H; auto.
+
+  rewrite Forall_forall; intros.
+  repeat nforall.
+  pose proof map_in_exists.
+  apply H0 in H as [y [FY INY]].
+  rewrite <- FY.
+  apply liftTT_insert. apply H10; auto.
+
+  unfold liftTE in *.
+  rewrite <- map_app.
+  apply IHx1; auto.
 Qed.
 
-
 Lemma type_kienv_weaken
- :  forall ke te x1 t1 k2
- ,  TYPE ke         te            x1            t1
- -> TYPE (ke :> k2) (liftTE 0 te) (liftTX 0 x1) (liftTT 0 t1).
+  : forall ds ke te x1 t1 k2,
+    TYPE ds ke te x1 t1
+ -> TYPE ds (ke :> k2) (liftTE 0 te) (liftTX 0 x1) (liftTT 0 t1).
 Proof.
  intros.
  assert (ke :> k2 = insert 0 k2 ke).
@@ -235,38 +517,113 @@ Qed.
    than this in the stack over the new one.
  *)
 Lemma type_tyenv_insert
- :  forall ke te ix x1 t1 t2
- ,  TYPE ke  te                x1            t1
- -> TYPE ke (insert ix t2 te) (liftXX ix x1) t1.
+  : forall ds ke te ix x1 t1 t2,
+    TYPE ds ke te x1 t1
+    -> TYPE ds ke (insert ix t2 te) (liftXX 1 ix x1) t1.
 Proof.
- intros. gen ix ke te t1 t2.
- induction x1; intros; simpl; inverts H; eauto.
+  intros. gen ds ix ke te t1 t2.
+  induction x1 using exp_mutind
+    with (PA := fun a => forall ds ke te ix tBuilds tRes t2,
+                    TYPEA ds ke te a tBuilds tRes
+                    -> TYPEA ds ke (insert ix t2 te) (liftXA 1 ix a) tBuilds tRes);
+    intros; invert_exp_type; simpl; eauto.
 
- Case "XVar".
+  Case "XVar".
   lift_cases; intros; auto.
 
- (* Case "XLAM". *)
- (*  apply TYLAM. simpl. *)
- (*  assert ( liftTE 0 (insert ix t2 te) *)
- (*         = insert ix (liftTT 0 t2) (liftTE 0 te)). *)
- (*   unfold liftTE. rewrite map_insert. auto. *)
- (*  rewrite H. *)
- (*  apply IHx1. auto. *)
+  (* Case "XLAM". *)
+  (*  apply TYLAM. simpl. *)
+  (*  assert ( liftTE 0 (insert ix t2 te) *)
+  (*         = insert ix (liftTT 0 t2) (liftTE 0 te)). *)
+  (*   unfold liftTE. rewrite map_insert. auto. *)
+  (*  rewrite H. *)
+  (*  apply IHx1. auto. *)
 
- Case "XLam".
+  Case "XLam".
   eapply TYLam.
-   auto.
-   rewrite insert_rewind. apply IHx1. auto.
+  auto.
+  rewrite insert_rewind. apply IHx1. auto.
+
+  Case "XTup".
+  eapply TYTup; eauto.
+  apply (Forall2_map_left (TYPE ds ke (insert ix t2 te))).
+  apply (Forall2_impl_in  (TYPE ds ke te)); eauto.
+  nforall. eauto.
+
+  (* Case "XProj". *)
+  (* eapply TYProj; eauto. spec IHx1 H5; eauto. *)
+  (* apply (Forall2_map_left (TYPE ds ke (insert ix t2 te))). *)
+  (* apply (Forall2_impl_in  (TYPE ds ke te)); eauto. *)
+  (* nforall. eauto. *)
+
+  Case "XNFun".
+  eapply TYNFun; eauto.
+  (* apply Forall_map. *)
+  (* eapply TYAlt; eauto. *)
+  rewrite insert_app. auto.
+
+  Case "XNApp".
+  eapply TYNApp; eauto.
+  apply (Forall2_map_left (TYPE ds ke (insert ix t2 te))).
+  apply (Forall2_impl_in  (TYPE ds ke te)); eauto.
+  nforall. eauto.
+
+  Case "XFix".
+  eapply TYFix; eauto.
+  repeat rewrite insert_rewind.
+  apply IHx1; auto.
+
+  Case "XCon".
+  eapply TYCon; eauto.
+  apply (Forall2_map_left (TYPE ds ke (insert ix t2 te))).
+  apply (Forall2_impl_in  (TYPE ds ke te)); eauto.
+  repeat nforall. eauto.
+
+  Case "XMatch".
+  eapply TYMatch; eauto.
+  apply Forall_map.
+  apply (Forall_impl_in (fun a => TYPEA ds ke te a (TCon tcPat) t1)); eauto.
+  repeat nforall. burn.
+
+  rewrite map_length; auto.
+
+  (* norm. *) repeat nforall.
+  intros. rename x into d.
+  rewrite map_map. unfold Basics.compose.
+  eapply map_exists_in.
+  have (In d (map dcOfAlt aa)).
+  assert (exists a, dcOfAlt a = d /\ In a aa).
+  eapply map_in_exists. auto.
+  shift a. rip.
+  eapply dcOfAlt_liftXA.
+
+  Case "XAlt".
+  eapply TYAlt; eauto.
+  rewrite insert_app. auto.
 Qed.
 
 
 Lemma type_tyenv_weaken
- :  forall ke te x1 t1 t2
- ,  TYPE ke  te         x1           t1
- -> TYPE ke (te :> t2) (liftXX 0 x1) t1.
+  : forall ds ke te x1 t1 t2,
+    TYPE ds ke te x1 t1
+    -> TYPE ds ke (te :> t2) (liftXX 1 0 x1) t1.
 Proof.
- intros.
- assert (te :> t2 = insert 0 t2 te).
+  intros.
+  assert (te :> t2 = insert 0 t2 te).
   destruct te; auto. rewrite H0.
   apply type_tyenv_insert. auto.
+Qed.
+
+Lemma type_tyenv_weaken_append
+  : forall ds ke te x1 t1 te',
+    TYPE ds ke te x1 t1
+    -> TYPE ds ke (te >< te') (liftXX (length te') 0 x1) t1.
+Proof.
+ intros.
+ induction te'; simpl.
+ rewrite liftXX_zero; auto.
+ rewrite <- nat_plus_one.
+ rrwrite (length te' + 1 = 1 + length te').
+ rewrite <- liftXX_plus.
+ eapply type_tyenv_weaken. auto.
 Qed.
