FiatFormal/Language/Base.v
@@ -9,3 +9,4 @@ Require Export Coq.Program.Basics.
 Require Export Coq.Arith.Compare_dec.
 
 Require Export FiatFormal.PMKTactics.
+Require Export FiatFormal.Tactics.
