FiatFormal/Language/SubstExpExp.v
@@ -6,58 +6,132 @@ Require Import FiatFormal.Language.TyJudge.
 
 (* Substitution of Values in Values preserves Typing ****************)
 Theorem subst_value_value_ix
- :  forall ix ke te x1 t1 x2 t2
- ,  get  ix te = Some t2
- -> TYPE ke te           x1 t1
- -> TYPE ke (delete ix te) x2 t2
- -> TYPE ke (delete ix te) (substXX ix x2 x1) t1.
+  : forall ds ix ke te x1 t1 x2 t2,
+    get ix te = Some t2
+    -> TYPE ds ke te           x1 t1
+    -> TYPE ds ke (delete ix te) x2 t2
+    -> TYPE ds ke (delete ix te) (substXX ix x2 x1) t1.
 Proof.
- intros. gen ix ke te t1 x2 t2.
- induction x1; intros; inverts H0; simpl; eauto.
+  intros. gen ds ix ke te t1 x2 t2.
+  induction x1 using exp_mutind
+    with (PA := fun a => forall ds ix ke te tsBuilds tRes x2 t2,
+                    get ix te = Some t2
+                    -> TYPEA ds ke te a tsBuilds tRes
+                    -> TYPE  ds ke (delete ix te) x2 t2
+                    -> TYPEA ds ke (delete ix te) (substXA ix x2 a) tsBuilds tRes);
+    intros; inverts H0; simpl; eauto.
 
- Case "XVar".
+  Case "XVar".
   fbreak_nat_compare.
   SCase "n = ix".
-   rewrite H in H3. inverts H3. auto.
+  rewrite H in H3. inverts H3. auto.
 
   SCase "n < ix".
-   apply TYVar.
-   rewrite <- H3. apply get_delete_above. auto. auto.
+  apply TYVar.
+  rewrite <- H3. apply get_delete_above. auto. auto.
 
   SCase "n > ix".
-   apply TYVar. auto.
-   rewrite <- H3.
-   destruct n.
-    burn.
-    simpl. nnat. apply get_delete_below. omega.
-    auto.
+  apply TYVar. auto.
+  rewrite <- H3.
+  destruct n.
+  burn.
+  simpl. nnat. apply get_delete_below. omega.
+  auto.
 
- (* Case "XLAM". *)
- (*  eapply (IHx1 ix) in H5. *)
- (*  apply TYLAM. *)
- (*   unfold liftTE. rewrite map_delete. eauto. *)
- (*   eapply get_map. eauto. *)
- (*   unfold liftTE. rewrite <- map_delete. *)
- (*    assert (map (liftTT 0) (delete ix te) = liftTE 0 (delete ix te)). *)
- (*     unfold liftTE. auto. rewrite H0. clear H0. *)
- (*    apply type_kienv_weaken. auto. *)
+  (* Case "XLAM". *)
+  (*  eapply (IHx1 ix) in H5. *)
+  (*  apply TYLAM. *)
+  (*   unfold liftTE. rewrite map_delete. eauto. *)
+  (*   eapply get_map. eauto. *)
+  (*   unfold liftTE. rewrite <- map_delete. *)
+  (*    assert (map (liftTT 0) (delete ix te) = liftTE 0 (delete ix te)). *)
+  (*     unfold liftTE. auto. rewrite H0. clear H0. *)
+  (*    apply type_kienv_weaken. auto. *)
 
- Case "XLam".
+  Case "XLam".
   apply TYLam.
-   auto.
-   rewrite delete_rewind.
-   eapply IHx1; eauto.
-   simpl. apply type_tyenv_weaken. auto.
+  auto.
+  rewrite delete_rewind.
+  eapply IHx1; eauto.
+  simpl. apply type_tyenv_weaken. auto.
+
+  Case "XTup".
+  apply TYTup.
+  apply (Forall2_map_left (TYPE ds ke (delete ix te))).
+  apply (Forall2_impl_in (TYPE ds ke te)); eauto.
+  nforall. intros.
+  eapply H; eauto.
+
+  Case "XNFun".
+  apply TYNFun; auto.
+  rewrite delete_app.
+  eapply IHx1; eauto.
+  rewrite <- delete_app.
+  eapply type_tyenv_weaken_append; auto.
+
+  Case "XNApp".
+  eapply TYNApp.
+  spec IHx1 H8.
+  eapply IHx1; eauto.
+  apply (Forall2_map_left (TYPE ds ke (delete ix te))).
+  apply (Forall2_impl_in (TYPE ds ke te)); eauto.
+  nforall. intros.
+  eapply H; eauto.
+
+  Case "XFix".
+  eapply TYFix; eauto.
+  repeat rewrite delete_rewind.
+  eapply IHx1; eauto.
+  simpl. pose proof (liftXX_plus 1 1).
+  rewrite <- H0.
+  repeat apply type_tyenv_weaken; auto.
+
+  Case "XCon".
+  eapply TYCon; eauto.
+  apply (Forall2_map_left (TYPE ds ke (delete ix te))).
+  apply (Forall2_impl_in  (TYPE ds ke te)); eauto.
+  repeat nforall; eauto.
+
+  Case "XMatch".
+  eapply TYMatch; eauto.
+  apply Forall_map.
+  apply (Forall_impl_in (fun x : alt => TYPEA ds ke (delete ix te) (substXA ix x2 x) (TCon tcPat) t1)).
+  repeat nforall; intros.
+  spec H H0. eauto.
+
+  repeat nforall; intros; eauto.
+  rewrite map_length; auto.
+
+(* norm. *) repeat nforall.
+  intros. rename x into d.
+  rewrite map_map. unfold Basics.compose.
+  eapply map_exists_in.
+  have (In d (map dcOfAlt aa)).
+  assert (exists a, dcOfAlt a = d /\ In a aa).
+  eapply map_in_exists. auto.
+  shift a. rip.
+  eapply dcOfAlt_substXA.
+
+
+  Case "XAlt".
+  assert (ts = map (substTT ix t2) ts).
+  apply simpleSubstMapEq; auto.
+  eapply TYAlt; eauto.
+  repeat nforall.
+  rewrite delete_app.
+  eapply IHx1; eauto.
+  rewrite <- delete_app.
+  eapply type_tyenv_weaken_append; auto.
 Qed.
 
 
 Theorem subst_value_value
- :  forall ke te x1 t1 x2 t2
- ,  TYPE ke (te :> t2) x1 t1
- -> TYPE ke te x2 t2
- -> TYPE ke te (substXX 0 x2 x1) t1.
+  : forall ds ke te x1 t1 x2 t2,
+    TYPE ds ke (te :> t2) x1 t1
+    -> TYPE ds ke te x2 t2
+    -> TYPE ds ke te (substXX 0 x2 x1) t1.
 Proof.
- intros.
- assert (te = delete 0 (te :> t2)). auto.
- rewrite H1. eapply subst_value_value_ix; eauto. eauto.
+  intros.
+  assert (te = delete 0 (te :> t2)). auto.
+  rewrite H1. eapply subst_value_value_ix; eauto. eauto.
 Qed.
