FiatFormal/Language/SubstTypeExp.v
@@ -10,56 +10,154 @@ Require Import FiatFormal.Language.SubstTypeType.
    to the result type.
  *)
 Theorem subst_type_exp_ix
- :  forall ix ke te x1 t1 t2 k2
- ,  get ix ke = Some k2
- -> TYPE ke  te x1 t1
+  : forall ix ds ke te x1 t1 t2 k2,
+    get ix ke = Some k2
+ -> TYPE ds ke te x1 t1
  -> KIND (delete ix ke)  t2 k2
- -> TYPE (delete ix ke)     (substTE ix t2 te)
-         (substTX ix t2 x1) (substTT ix t2 t1).
+ -> TYPE ds (delete ix ke)     (substTE ix t2 te)
+           (substTX ix t2 x1) (substTT ix t2 t1).
 Proof.
- intros. gen ix ke te t1 t2 k2.
- induction x1; intros; simpl; inverts H0; eauto.
+  intros. gen ix ds ke te t1 t2 k2.
+  induction x1 using exp_mutind
+    with (PA := fun a => forall ix ds ke te tBuilds tRes t2 k2, (* dc tsArgs x, *)
+                    get ix ke = Some k2
+                    -> TYPEA ds ke te a (* (AAlt dc tsArgs x) *) tBuilds tRes
+                    -> KIND (delete ix ke) t2 k2
+                    -> TYPEA ds (delete ix ke) (substTE ix t2 te)
+                            (substTA ix t2 a (* (AAlt dc tsArgs x) *)) (substTT ix t2 tBuilds) (substTT ix t2 tRes));
+    intros; simpl; inverts H0; eauto.
 
- Case "XVar".
+  Case "XVar".
   apply TYVar.
   unfold substTE. eapply get_map. auto.
   eapply subst_type_type_ix; eauto.
 
- (* Case "XLAM". *)
- (*  simpl. apply TYLAM. *)
- (*  rewrite delete_rewind. *)
- (*  rewrite (liftTE_substTE 0 ix). *)
- (*  eapply IHx1; eauto. *)
- (*   apply liftTT_weaken. auto. *)
+  (* Case "XLAM". *)
+  (*  simpl. apply TYLAM. *)
+  (*  rewrite delete_rewind. *)
+  (*  rewrite (liftTE_substTE 0 ix). *)
+  (*  eapply IHx1; eauto. *)
+  (*   apply liftTT_weaken. auto. *)
 
- (* Case "XAPP". *)
- (*  rewrite (substTT_substTT 0 ix). *)
- (*  apply TYAPP. *)
- (*   simpl. eapply (IHx1 ix) in H6; eauto. *)
- (*   simpl. eapply subst_type_type_ix; eauto. *)
+  (* Case "XAPP". *)
+  (*  rewrite (substTT_substTT 0 ix). *)
+  (*  apply TYAPP. *)
+  (*   simpl. eapply (IHx1 ix) in H6; eauto. *)
+  (*   simpl. eapply subst_type_type_ix; eauto. *)
 
- Case "XLam".
+  Case "XLam".
   simpl. apply TYLam.
   eapply subst_type_type_ix; eauto.
   unfold substTE. rewrite map_rewind.
   assert ( map (substTT ix t2) (te :> t)
-         = substTE ix t2 (te :> t)). auto.
+           = substTE ix t2 (te :> t)). auto.
   rewrite H0.
-   eapply IHx1; eauto.
+  eapply IHx1; eauto.
 
- Case "XApp".
+  Case "XApp".
   eapply TYApp.
-   eapply IHx1_1 in H6; eauto.
-   eapply IHx1_2 in H8; eauto.
+  eapply IHx1_1 in H7; eauto.
+  eapply IHx1_2 in H9; eauto.
+
+  Case "XTup".
+  apply TYTup.
+  apply (Forall2_map_left (TYPE ds (delete ix ke) (substTE ix t2 te))).
+  apply (Forall2_map_right (fun (x : exp) (y : ty) => TYPE ds (delete ix ke) (substTE ix t2 te) (substTX ix t2 x) y)).
+  apply (Forall2_impl_in (TYPE ds ke te)); eauto.
+  nforall. intros.
+  eapply H; eauto.
+
+  Case "XProj".
+  eapply TYProj; simpl; eauto.
+  spec IHx1 H7. simpl in *; eauto.
+
+  Case "XNFun".
+  eapply TYNFun; eauto.
+  apply Forall_map.
+  repeat nforall; intros.
+  eapply subst_type_type_ix; eauto.
+  spec IHx1 H9.
+  unfold substTE in *.
+  rewrite <- map_app; eauto.
+
+  Case "XNApp".
+  apply TYNApp with (ts := map (substTT ix t2) ts).
+  assert (substTT ix t2 (TNFun ts t1) = TNFun (map (substTT ix t2) ts) (substTT ix t2 t1)) by auto.
+  rewrite <- H0.
+  eapply IHx1; eauto.
+  apply (Forall2_map_left (TYPE ds (delete ix ke) (substTE ix t2 te))).
+  apply (Forall2_map_right (fun (x : exp) (y : ty) => TYPE ds (delete ix ke) (substTE ix t2 te) (substTX ix t2 x) y)).
+  apply (Forall2_impl_in  (TYPE ds ke te)); eauto.
+  nforall. intros.
+  eapply H; eauto.
+
+  Case "XFix".
+  eapply TYFix. eapply subst_type_type_ix; eauto.
+  unfold substTE in *.
+  assert (substTT ix t3 (TFun t1 t2) = (TFun (substTT ix t3 t1) (substTT ix t3 t2))) by auto.
+  rewrite <- H0.
+  repeat rewrite <- map_cons.
+  eapply IHx1; eauto.
+
+  Case "XCon".
+  eapply TYCon; eauto.
+  apply (Forall2_map_left (TYPE ds (delete ix ke) (substTE ix t2 te))).
+  apply (Forall2_impl_in  (TYPE ds ke te)); eauto.
+  nforall; eauto.
+  intros. spec H7 H3.
+  assert (y = substTT ix t2 y).
+  apply simpleSubstEq; auto.
+  rewrite H8.
+  nforall.
+  eapply H; eauto.
+
+  Case "XMatch".
+  eapply TYMatch; eauto.
+  assert (TCon tcPat = (substTT ix t2 (TCon tcPat))) by auto.
+  rewrite H0.
+  eapply IHx1; eauto.
+
+  apply Forall_map.
+  apply (Forall_impl_in (fun a => TYPEA ds ke te a (TCon tcPat) t1)); eauto.
+  repeat nforall; intros.
+  spec H H0. spec H H1. spec H H3. eauto.
+  rewrite map_length; auto.
+
+  (* norm. *) repeat nforall.
+  intros. rename x into d.
+  rewrite map_map. unfold Basics.compose.
+  eapply map_exists_in.
+  have (In d (map dcOfAlt aa)).
+  assert (exists a, dcOfAlt a = d /\ In a aa).
+  eapply map_in_exists. auto.
+  shift a. rip.
+  eapply dcOfAlt_substTA.
+
+  Case "XAlt".
+  assert (ts = map (substTT ix t2) ts).
+  apply simpleSubstMapEq; auto.
+  eapply TYAlt; eauto.
+  rewrite <- H0; auto.
+  rewrite <- H0; auto.
+
+  apply Forall_map.
+
+  rewrite Forall_forall; intros.
+  repeat nforall.
+  eapply subst_type_type_ix; eauto.
+
+  unfold substTE in *.
+  rewrite <- map_app.
+  eapply IHx1; eauto.
 Qed.
 
 
 Theorem subst_type_value
- :  forall ke te x1 t1 t2 k2
- ,  TYPE (ke :> k2) te x1 t1
- -> KIND ke  t2 k2
- -> TYPE ke                (substTE 0 t2 te)
-         (substTX 0 t2 x1) (substTT 0 t2 t1).
+  : forall ds ke te x1 t1 t2 k2,
+    TYPE ds (ke :> k2) te x1 t1
+    -> KIND ke  t2 k2
+    -> TYPE ds ke (substTE 0 t2 te)
+           (substTX 0 t2 x1) (substTT 0 t2 t1).
 Proof.
  intros.
  assert (ke = delete 0 (ke :> k2)). auto. rewrite H1.
